unity/scheduling/infinite.lean
@@ -44,7 +44,7 @@ structure sch_state :=
   (queue : rrobin lbl)
   (inv : sch.current (t.req target) queue ∈ t.req target)
 
-def sch_state.req (s : sch_state) : set lbl :=
+def req (s : sch_state) : set lbl :=
 t.req s.target
 
 lemma first_mem {s : t.σ}
@@ -60,8 +60,8 @@ end
 
 noncomputable def shift (s : sch_state)
 : rrobin lbl :=
-if h : first s.req s.queue < succ s.q_len
-then s.queue ∘ bijection.rotate_right' (first s.req s.queue) (succ s.q_len) h
+if h : first (req s) s.queue < succ s.q_len
+then s.queue ∘ bijection.rotate_right' (first (req s) s^.queue) (succ s.q_len) h
 else s.queue
 
 lemma sch.select_inv
@@ -81,7 +81,7 @@ def sch.first : sch_state :=
 
 noncomputable def sch.step (s : sch_state) : sch_state :=
 { q_len := s.q_len + 1
-, target := t.next (sch.current s.req s.queue) s.target s.inv
+, target := t.next (sch.current (req s) s.queue) s.target s.inv
 , queue := shift s
 , inv := sch.select_inv _ _ }
 
@@ -92,7 +92,7 @@ noncomputable def scheduler : program sch_state :=
 open sch_state has_mem
 
 noncomputable def next (s : sch_state) : lbl :=
-sch.current s.req s.queue
+sch.current (req s) s.queue
 
 def rank (l : lbl) (s : sch_state) : ℕ := s.queue.g l + (s.queue.g l - s.q_len)
 
@@ -101,7 +101,7 @@ lemma pending_not_move (s : sch_state) (l : lbl)
 : ((sch.step s).queue).g l = s.queue.g l :=
 begin
   unfold sch.step sch_state.queue shift,
-  cases decidable.em (first s.req s.queue < succ s.q_len) with h' h',
+  cases decidable.em (first (req t s) s.queue < succ s.q_len) with h' h',
   { rw [dif_pos h',comp_g],
     unfold comp,
     rw bijection.rotate_right'_g_eq_of_ge_j _ h' h, },
@@ -109,12 +109,12 @@ begin
 end
 
 lemma shift_down (s : sch_state) (l : lbl)
-  (h₀ : first s.req s.queue < s.queue.g l)
+  (h₀ : first (req s) s.queue < s.queue.g l)
   (h₁ : s.queue.g l < succ s.q_len)
 : succ (((sch.step s).queue).g l) = s.queue.g l :=
 begin
   unfold sch.step sch_state.queue shift,
-  note h : first s.req s.queue < succ s.q_len := lt_trans h₀ h₁,
+  have h : first (req t s) s.queue < succ s.q_len := lt_trans h₀ h₁,
   rw [dif_pos h,comp_g], unfold comp,
   rw bijection.succ_rotate_right'_g_eq_self (s.queue.g l) _ h₀ h₁,
 end
@@ -124,11 +124,11 @@ lemma q_len_inc (s : sch_state)
 by { rw -add_one_eq_succ, refl }
 
 lemma not_req_not_move (s : sch_state) (l : lbl)
-  (h : s.queue.g l < first s.req s.queue)
+  (h : s.queue.g l < first (req s) s.queue)
 : (sch.step s).queue.g l = s.queue.g l :=
 begin
   unfold sch.step sch_state.queue shift,
-  cases decidable.em (first s.req s.queue < succ s.q_len) with h' h',
+  cases decidable.em (first (req t s) s.queue < succ s.q_len) with h' h',
   { rw [dif_pos h',comp_g],
     unfold comp,
     rw [bijection.rotate_right'_g_eq_of_lt_i _ _ h], },
@@ -136,8 +136,8 @@ begin
 end
 
 lemma not_mem_req {s : sch_state} {l : lbl}
-  (h : first (sch_state.req s) s.queue > s.queue.g l)
-: l ∉ s.req :=
+  (h : first (req s) s.queue > s.queue.g l)
+: l ∉ req s :=
 begin
   intro h',
   revert h,
@@ -150,12 +150,12 @@ begin
 end
 
 lemma le_rank_of_lt_first {s : sch_state} {l : lbl}
-  (Hgt : s.queue.g l < first (sch_state.req s) s.queue)
+  (Hgt : s.queue.g l < first (req s) s.queue)
 : rank l (sch.step s) ≤ rank l s :=
 begin
   unfold rank,
   cases le_or_gt (s.queue.g l) (s.q_len) with h h,
-  { note h' : s.queue.g l ≤ succ s.q_len := le_succ_of_le h,
+  { have h' : s.queue.g l ≤ succ s.q_len := le_succ_of_le h,
     rw [not_req_not_move _ _ _ Hgt,q_len_inc
        ,sub_eq_zero_of_le h,sub_eq_zero_of_le h'] },
   { rw [pending_not_move _ _ _ h,q_len_inc],
@@ -165,13 +165,13 @@ begin
 end
 
 lemma lt_rank_of_gt_first {s : sch_state} {l : lbl}
-  (Hlt : first (sch_state.req s) (s.queue) < (s.queue).g l)
+  (Hlt : first (req s) (s.queue) < (s.queue).g l)
 : rank l (sch.step s) < rank l s :=
 begin
   unfold rank,
-  cases le_or_gt s.q_len (first s.req s.queue) with h h,
+  cases le_or_gt s.q_len (first (req t s) s.queue) with h h,
     -- h : s.q_len ≤ first (sch_state.req s) (s.queue)
-  { note h' : s.q_len < s.queue.g l := lt_of_le_of_lt h Hlt,
+  { have h' : s.q_len < s.queue.g l := lt_of_le_of_lt h Hlt,
     rw [pending_not_move _ _ _ h'],
     unfold sch.step sch_state.q_len,
     rw [add_one_eq_succ,-nat.add_sub_assoc h'
@@ -232,11 +232,11 @@ begin
   intros σ Heq Hnnext,
   simp, simp at Heq,
   cases Heq with Heq Hmem,
-  note HH := eq_next_or_rank_eq_or_rank_lt _ v Heq,
+  have HH := eq_next_or_rank_eq_or_rank_lt _ v Heq,
   rw or_iff_not_imp at HH,
   simp [not_or_iff_not_and_not] at Hnnext,
-  note Hnnext' : ¬ l = next t σ := Hnnext.left,
-  note HH' := HH Hnnext',
+  have Hnnext' : ¬ l = next t σ := Hnnext.left,
+  have HH' := HH Hnnext',
   rw [or_iff_not_imp,not_and_iff_not_or_not,not_not_iff_self] at HH',
   right, apply HH', clear HH' HH,
   apply or.intro_left _ Hmem,
@@ -269,7 +269,7 @@ end
 lemma STEP
 : co' scheduler
     (λ (σ σ' : sch_state),
-       ∃P, σ'.target = t.next (sch.current σ.req σ.queue) σ.target P) :=
+       ∃P, σ'.target = t.next (sch.current (req σ) σ.queue) σ.target P) :=
 begin
   unfold co',
   intros σ σ',
